theory/System/PathORAMDef.v
@@ -1,5 +1,7 @@
 Require Import Coq.Lists.List.
 Import ListNotations.
+Require Import POram.Utils.Classes.
+Import MonadNotation.
 Require Import Coq.Classes.EquivDec.
 Require Import POram.Utils.Rationals.
 Require Import POram.Utils.Tree.
@@ -7,6 +9,7 @@ Require Import POram.Utils.Lists.
 Require Import POram.Utils.Classes.
 Require Import POram.Utils.StateT.
 Require Import POram.Utils.Distributions.
+Require Import POram.Utils.NoDup.
 (*** PATH ORAM ***)
 
 (** 
@@ -68,135 +71,243 @@ Class Config: Type :=
 Section PORAM.
   Context `{Config}.
   
-Definition block_id := nat.
-Record block : Type := Block
-  { block_blockid : block_id
-  ; block_payload : nat
-  }.
-Definition position_map := dict block_id path.
-Definition stash := list block.
-Definition bucket := list block.
+  Definition block_id := nat.
+  Record block : Type := Block
+                           { block_blockid : block_id
+                           ; block_payload : nat
+                           }.
+  Definition position_map := dict block_id path.
+  Definition stash := list block.
+  Definition bucket := list block.
 
-Definition oram : Type := tree (option bucket).
+  Definition oram : Type := tree (option bucket).
 
-Record state : Type := State
-  { state_position_map : position_map
-  ; state_stash : stash
-  ; state_oram : oram
-  }.
+  Record state : Type := State
+                           { state_position_map : position_map
+                           ; state_stash : stash
+                           ; state_oram : oram
+                           }.
 
-Inductive operation := 
+  Inductive operation := 
   | Read : operation 
   | Write : nat -> operation.
 
-Definition Poram : Type -> Type :=
-  StateT state dist.
+  Definition Poram : Type -> Type :=
+    StateT state dist.
 
-Fixpoint lookup_path_oram (o : oram) : path -> list bucket :=
-  match o with
-  | leaf => fun _ => []
-  | node obkt o_l o_r =>
-      fun p => 
-        match p with
-        | [] =>
-            match obkt with
-            | Some bkt => [bkt]
-            | None => []
-            end
-        | h :: t =>
-            match h with
-            | true => match obkt with
-                     | Some bkt => bkt :: lookup_path_oram o_l t
-                     | None => lookup_path_oram o_l t
-                     end
-            | false => match obkt with
-                      | Some bkt => bkt :: lookup_path_oram o_r t
-                      | None => lookup_path_oram o_r t
-                      end
-            end
+  Fixpoint lookup_path_oram (o : oram) : path -> list bucket :=
+    match o with
+    | leaf => fun _ => []
+    | node obkt o_l o_r =>
+        fun p => 
+          match p with
+          | [] =>
+              match obkt with
+              | Some bkt => [bkt]
+              | None => []
+              end
+          | h :: t =>
+              match h with
+              | true => match obkt with
+                       | Some bkt => bkt :: lookup_path_oram o_l t
+                       | None => lookup_path_oram o_l t
+                       end
+              | false => match obkt with
+                        | Some bkt => bkt :: lookup_path_oram o_r t
+                        | None => lookup_path_oram o_r t
+                        end
+              end
+          end
+    end.
+
+  Fixpoint clear_path (o : oram ) : path -> oram :=
+    match o with
+    | leaf => fun _ => leaf
+    | node obkt o_l o_r =>
+        fun p =>
+          match p with
+          | [] => node None o_l o_r
+          | h :: t =>
+              match h with
+              | true => node None (clear_path o_l t) o_r
+              | false => node None o_l (clear_path o_r t)
+              end
+          end
+    end.
+
+  Fixpoint makeBoolList (b : bool) (n : nat) : list bool :=
+    match n with
+    | O => []
+    | S m => b :: makeBoolList b m
+    end.
+
+  Definition calc_path (id : block_id) (s : state):=
+    let l := LOP in 
+    lookup_dict (makeBoolList false l) id (state_position_map s).
+
+  Definition blk_in_p (id : block_id) (v : nat) (o : oram) (p: path) := 
+    let path_blks := concat(lookup_path_oram o p) in
+    In (Block id v) path_blks.
+
+  Definition blk_in_path (id : block_id) (v : nat) (s : state): Prop :=
+    blk_in_p id v (state_oram s) (calc_path id s).
+
+  Scheme Equality for list.
+  Definition isEqvPath (p1 p2 : path) (idx : nat) : bool := list_beq bool Bool.eqb  (takeL idx p1) (takeL idx p2).
+
+  Fixpoint get_cand_bs (h : stash)(p : path)(stop : nat)(m : position_map) : list block :=
+    match h with
+    | [] => []
+    | x :: xs =>
+        let l := LOP in 
+        let rhs_path := lookup_dict (makeBoolList false l) (block_blockid x) m in
+        if @isEqvPath p rhs_path stop 
+        then x :: get_cand_bs xs p stop m 
+        else get_cand_bs xs p stop m 
+    end. 
+
+  (* n is the capability of each node, the current magic number is 4 based on the original paper *)
+
+  Definition get_write_back_blocks (p : path) (h : stash) (n : nat)(lvl : nat) (mp : position_map ) : list block :=
+    match (length h) with
+    | O => []
+    | S m => let cand_bs := get_cand_bs h p lvl mp in
+            takeL (Nat.min (length cand_bs) n ) cand_bs
+    end.
+
+
+    Scheme Equality for nat.
+  Fixpoint remove_aux (lst : list block) (x : block) : list block :=
+    match lst with
+    | [] => []
+    | h :: t => 
+        if andb (Nat.eqb (block_blockid h) (block_blockid x))
+             (Nat.eqb (block_payload h) (block_payload x))
+        then t 
+        else h :: (remove_aux t x)
+    end.
+
+  Fixpoint remove_list_sub (sublist : list block) (lst : list block) : list block :=
+    match sublist with
+    | [] => lst
+    | h :: t => remove_list_sub t (remove_aux lst h)
+    end.
+  
+  Fixpoint lookup_ret_data (id : block_id) (lb : list block): nat :=
+    match lb with
+    | [] => 0
+    | h :: t =>
+        if Nat.eqb (block_blockid h) id then block_payload (h%nat)
+        else lookup_ret_data id t
+    end.
+
+  Definition up_oram_tr (o : oram) (stop : nat) (d_n : bucket)
+    (p : path) : oram :=
+    update_tree o stop (Some d_n) p.
+  
+  Definition blocks_selection (p : path) (lvl : nat) (s : state ) : state :=
+    (* unpack the state *)
+    let m := state_position_map s in (* pos_map *) 
+    let h := state_stash s in        (* stash *)
+    let o := state_oram s in         (* oram tree *)
+    let wbs := get_write_back_blocks p h 4 lvl m in (* 4 is the capability of the bucket or equivalently the number of blocks the bucket holds *)
+    let up_h := remove_list_sub wbs h in 
+    let up_o := up_oram_tr o lvl wbs p in
+    (State m up_h up_o).
+
+  (* write_back is the last for-loop, searching backwards from the bottom of the tree to seek empty slots to write candidcate blocs back *)
+
+  Fixpoint write_back (s : state) (p : path) (lvl : nat) : state := 
+    match lvl with
+    | O => s 
+    | S m => write_back (blocks_selection p m s) p m
+    end.
+
+  Fixpoint iterate_right {X} (start : nat) (p : path) (f : path -> nat -> X -> X) (n : nat) (x : X) : X :=
+    match n with
+    | O => x
+    | S m => f p start (iterate_right (S start) p f m x)
+    end.
+
+    Fixpoint get_all_blks_tree (o : oram) : list block :=
+    match o with
+    | leaf => []
+    | node obkt o_l o_r => 
+        match obkt with
+        | None => get_all_blks_tree o_l ++ get_all_blks_tree o_r
+        | Some bkt => bkt ++ (get_all_blks_tree o_l ++ get_all_blks_tree o_r)
         end
-  end.
+    end.
 
-Fixpoint clear_path (o : oram ) : path -> oram :=
-  match o with
-  | leaf => fun _ => leaf
-  | node obkt o_l o_r =>
-      fun p =>
-        match p with
-        | [] => node None o_l o_r
-        | h :: t =>
-            match h with
-            | true => node None (clear_path o_l t) o_r
-            | false => node None o_l (clear_path o_r t)
-            end
-        end
-  end.
+  Definition write_back_r (start : nat) (p : path) (step : nat) (s : state):=
+    iterate_right start p blocks_selection step s.
 
-Fixpoint makeBoolList (b : bool) (n : nat) : list bool :=
-  match n with
-  | O => []
-  | S m => b :: makeBoolList b m
-  end.
+    Definition get_pre_wb_st (id : block_id) (op : operation) (m : position_map) (h : stash ) (o : oram) (p p_new: path) :=
+    let m' := update_dict id p_new m in
+    let bkts := lookup_path_oram o p in
+    let bkt_blocks := concat bkts in
+    let h' := bkt_blocks ++ h in
+    let h'' := remove_list 
+                 (fun blk => (Nat.eqb (block_blockid blk) id)) h' in  
+    let h''' :=
+      match op with
+      | Read => h'
+      | Write d => (Block id d) ::  h''
+      end in
+    let o' := clear_path o p in 
+    State m' h''' o'.
 
-Definition calc_path (id : block_id) (s : state):=
-  let l := LOP in 
-  lookup_dict (makeBoolList false l) id (state_position_map s).
+  Definition get_post_wb_st (s : state) (id_path : path):=
+    write_back_r O id_path (length id_path) s.
+  
+  Definition get_ret_data (id : block_id)(h : stash)(p : path) (o : oram):=
+    let bkts := lookup_path_oram o p in
+    let bkt_blocks := concat bkts in
+    let h' := bkt_blocks ++ h in
+    let ret_data := lookup_ret_data id h' in
+    ret_data. 
 
-Definition blk_in_p (id : block_id) (v : nat) (o : oram) (p: path) := 
-  let path_blks := concat(lookup_path_oram o p) in
-  In (Block id v) path_blks.
+  Definition access (id : block_id) (op : operation) :
+    Poram (path * nat) :=
+    PST <- get ;;
+    (* unpack the state *)
+    let m := state_position_map PST in
+    let h := state_stash  PST in
+    let o := state_oram PST in 
+    (* get path for the index we are querying *)
+    let len_m := LOP in
+    let p := lookup_dict (makeBoolList false len_m) id m in
+    (* flip a bunch of coins to get the new path *)      
+    p_new <- liftT (coin_flips len_m) ;;
+    (* get the updated path oram state to put and the data to return *)
+    let n_st := get_post_wb_st (get_pre_wb_st id op m h o p p_new) p in
+    let ret_data := get_ret_data id h p o in
+    (* put the updated state back *)
+    _ <- put n_st ;;
+    (* return the path l and the return value *)
+    mreturn((p, ret_data)).
 
-Definition blk_in_path (id : block_id) (v : nat) (s : state): Prop :=
-  blk_in_p id v (state_oram s) (calc_path id s).
-
-Scheme Equality for list.
-Definition isEqvPath (p1 p2 : path) (idx : nat) : bool := list_beq bool Bool.eqb  (takeL idx p1) (takeL idx p2).
-
-Fixpoint get_cand_bs (h : stash)(p : path)(stop : nat)(m : position_map) : list block :=
-  match h with
-  | [] => []
-  | x :: xs =>
-      let l := LOP in 
-      let rhs_path := lookup_dict (makeBoolList false l) (block_blockid x) m in
-      if @isEqvPath p rhs_path stop 
-      then x :: get_cand_bs xs p stop m 
-      else get_cand_bs xs p stop m 
-  end. 
-
-(* n is the capability of each node, the current magic number is 4 based on the original paper *)
-
-Definition get_write_back_blocks (p : path) (h : stash) (n : nat)(lvl : nat) (mp : position_map ) : list block :=
-  match (length h) with
-  | O => []
-  | S m => let cand_bs := get_cand_bs h p lvl mp in
-          takeL (Nat.min (length cand_bs) n ) cand_bs
-  end.
-
-
-
-
-
-
-
-
-
-
-
-
-
-
-
-
-
-
-
-
-
-
-
-
-
-
+    Record well_formed (s : state ) : Prop := 
+    {
+      no_dup_stash : NoDup (List.map block_blockid (state_stash s)); 
+      no_dup_tree : NoDup (List.map block_blockid (get_all_blks_tree (state_oram s)));
+      tree_stash_disj : disjoint_list (List.map block_blockid (get_all_blks_tree (state_oram s)))
+                          (List.map block_blockid (state_stash s)); 
+      is_pb_tr : is_p_b_tr (state_oram s) (S LOP);
+      blk_in_path_in_tree :
+      forall id, 
+        let m := state_position_map s in
+        let p := lookup_dict (makeBoolList false LOP) id m in
+        let o := state_oram s in 
+        let bkts := lookup_path_oram o p in
+        let bkt_blocks := concat bkts in
+        In id (List.map block_blockid (get_all_blks_tree o)) ->
+        In id (List.map block_blockid bkt_blocks);
+      path_length : 
+      let m := (state_position_map s) in
+      let len_m := LOP in 
+      forall id, length(lookup_dict (makeBoolList false len_m) id m) = LOP;
+    }.
 
 
 
